src/casemate-check-rocq/theories/utils.v
@@ -73,6 +73,7 @@ Definition b0 := BV64 0.
 Definition b1 := BV64 1.
 Definition b2 := BV64 2.
 Definition b3 := BV64 3.
+Definition b4 := BV64 4.
 Definition b7 := BV64 7.
 Definition b8 := BV64 8.
 Definition b12 := BV64 12.
@@ -85,33 +86,38 @@ Definition b1023 := BV64 1023.
 (** Addresses **)
 
 Inductive thread_identifier :=
-| Thread_identifier : nat -> thread_identifier
+| TID : u64 -> thread_identifier
 .
 Global Instance thread_identifier_eq_decision : EqDecision thread_identifier.
   Proof. solve_decision. Qed.
 
+Definition thread_identifier_to_val (tid : thread_identifier) : u64 :=
+  match tid with
+  | TID val => val
+  end.
+
 Inductive phys_addr_t :=
-| Phys_addr : u64 -> phys_addr_t
+| PA : u64 -> phys_addr_t
 .
 
 Global Instance phys_addr_t_eq_decision : EqDecision phys_addr_t.
   Proof. solve_decision. Qed.
 
-Definition phys_addr_val (root : phys_addr_t) : u64 :=
-  match root with
-    | Phys_addr r => r
-  end
-.
+Definition phys_addr_val (phys_addr : phys_addr_t) : u64 :=
+  match phys_addr with
+  | PA val => val
+  end.
+
 Definition pa_plus (a b : phys_addr_t) : phys_addr_t :=
-  Phys_addr ((phys_addr_val a) b+ (phys_addr_val b))
+  PA ((phys_addr_val a) b+ (phys_addr_val b))
 .
 Infix "pa+" := pa_plus (at level 50).
 Definition pa_mul (a b : phys_addr_t) : phys_addr_t :=
-  Phys_addr ((phys_addr_val a) b* (phys_addr_val b))
+  PA ((phys_addr_val a) b* (phys_addr_val b))
 .
 Infix "pa*" := pa_mul (at level 40).
 Notation "<[ K := V ]> D" := (<[ bv_shiftr_64 (phys_addr_val K) b3 := V ]> D) (at level 100).
-Definition pa0 := Phys_addr b0.
+Definition pa0 := PA b0.
 
 Inductive sm_owner_t :=
 | Root : phys_addr_t -> sm_owner_t
@@ -128,6 +134,15 @@ Definition root_val (root : sm_owner_t) : phys_addr_t :=
 Inductive entry_stage_t :=
   | S1
   | S2
+.
+
+Inductive vmid_t :=
+   | U64 : u64 -> vmid_t
+ .
+
+Inductive addr_id_t :=
+  | ASID : u64 -> addr_id_t
+  | VMID : u64 -> addr_id_t
 .
 
 Inductive result (A B: Type): Type :=
@@ -148,3 +163,19 @@ Inductive internal_error_type :=
   | IET_no_write_authorization
 .
 
+Fixpoint nth_opt {A : Type} (n : nat) (l : list A) {struct l} : option A :=
+  match n, l with
+  | O, x :: l' => Some x
+  | O, _ => None
+  | S m, nil => None
+  | S m, x :: t => nth_opt m t
+  end.
+
+Fixpoint idx_of {A : Type} (f : A -> bool) (acc : nat) (l : list A) {struct l} : nat :=
+  match l with
+  | nil => acc
+  | x :: l' => if (f x) then acc else idx_of f (acc + 1) l'
+  end.
+
+Definition index_of {A : Type} (f : A -> bool) (l : list A) : nat :=
+  idx_of f 0 l.
